simulation of beta reduction

LJm/FragmentLambda.v
@@ -245,19 +245,21 @@ Theorem typing_preserved2 G t A : typingT G t A -> forall H : is_lambda t, typin
 Admitted.
 
 
-(************************
-*** simulation of Stlc beta 
-*************************)
+(********
+ * Simulation of Stlc beta reduction by LJm beta1 reduction --only one step so far
+ ********)
 
-(* below is a copy of the beta relation from STLC *)
+(* Definition of beta rule adapted from Stlc --in Stlc it already comes together with cbn closure *)
 
 Inductive beta : exp -> exp -> Prop :=
  | beta_base : forall (e1 e2:exp),
      lc_exp (S.abs e1) ->
      lc_exp e2 ->
-     beta (S.app (S.abs e1) e2) (open e1 e2).
+     beta (S.app  (S.abs e1) e2)  (open e1 e2).
 
 Hint Constructors beta.
+
+(*The lemmata that follow lead to the thm on the simulation of a beta step at STLC by a beta1 step in lJm*)
 
 Lemma lcT_from_lc_exp : forall e, lc_exp e -> lcT (exp_to_terms e).
 Proof.
@@ -271,55 +273,112 @@ Qed.
 
 Lemma bv_zero : forall n, lcT (abs (var_b n)) -> n=0.
 Proof.
-  intros. inversion H. pick fresh x. specialize (H1 x). cbn in H1. destruct (lt_eq_lt_dec n 0).
+  intros. inversion H. pick fresh x.  specialize (H1 x). cbn in H1. destruct (lt_eq_lt_dec n 0).
   - destruct s.
     + inversion H1.
     + trivial.
   - inversion H1.
 Qed.
 
-Theorem sim_by_beta_term: forall e1 e2,   beta e1 e2 -> beta1T 
-(exp_to_terms e1) (exp_to_terms e2).
+
+(* Simulation of the beta rule ---without compatible closure --by beta1 of LJm *)
+
+Lemma sim_by_beta_term : forall e1 e2,
+    beta e1 e2 -> beta1T (exp_to_terms e1) (exp_to_terms e2).
 Proof.
    intros. inversion H. simpl.  subst. rewrite  commut_opens. constructor.
-   - constructor. intro. inversion H0.
-     change ( lcT (openT (exp_to_terms e0) (exp_to_terms (S.var_f x)))).
-     rewrite <- commut_opens. specialize H3 
+   - constructor. intro. inversion H0. change ( lcT (openT (exp_to_terms 
+e0) (exp_to_terms (S.var_f x)))). rewrite <- commut_opens. specialize H3 
 with x. apply lcT_from_lc_exp. trivial.
    - apply lcT_from_lc_exp. trivial.
    - constructor. intro. cbn.  trivial.
 Qed.
 
-Lemma term_to_exp_commutes_open: forall e1 e2
-(H1:is_lambda e1) (H2:is_lambda e2) (H:is_lambda (openT e2 e1)),
-term_to_exp (open_term_wrt_term_rec 0 e1 e2) H =
-open (term_to_exp e2 H2)(term_to_exp e1 H1).
-Admitted.
 
-Lemma term_to_exp_preserves_lc: forall t H, lcT t -> lc_exp(term_to_exp t H).
-  intros.
-  inversion H; subst; cbn; trivial.
-  - inversion H0.
-  - inversion H0; subst.
-    constructor; intro.
-Admitted.
 
-Theorem term_to_exp_preserves_beta1: forall e1 e2,
-forall (H1:is_lambda e1) (H2:is_lambda e2),
-beta1T e1 e2 -> beta (term_to_exp e1 H1) (term_to_exp e2 H2).
+
+(* Definition of full compatible closure of beta ---not in Stlc   *)
+
+Inductive ccBeta : exp -> exp -> Prop :=
+ | ccBbase : forall (e1 e2:exp),
+     beta e1 e2 ->
+     ccBeta e1 e2
+ | ccBapp1 : forall (e1 e2 e:exp),
+     ccBeta e1 e2 -> lc_exp e ->
+     ccBeta (S.app e1 e) (S.app e2 e)
+ | ccBapp2 : forall (e1 e2 e:exp),
+     ccBeta e1 e2 -> lc_exp e ->
+     ccBeta (S.app e e1) (S.app e e2)
+ | ccBabs : forall (e1 e2:exp) (L:vars),
+     (forall (x:var), x `notin` L ->
+                 ccBeta (open e1 (S.var_f x))  (open e2 (S.var_f x))) ->
+     ccBeta (S.abs e1) (S.abs e2).
+
+Hint Constructors ccBeta.
+
+(* assumes from the base relation one can conclude local closedness for both terms *)
+(* NOTE: the definition below should eventualy replace the one in LJm Definitions.v 
+  and the proofs bellow adjusted by adding the prefix Definitions. *)
+Inductive ccRTT (R : term -> term -> Prop) : term -> term -> Prop :=
+ | cc_base : forall (t t':term),
+     R t t' -> ccRTT R t t'
+ | cc_abs : forall (t t':term) (L:vars),
+     (forall (x:var), x `notin` L ->
+     ccRTT R (openT t (var_f x))  (openT t' (var_f x))) -> ccRTT R (abs t) (abs t')
+ | cc_app1 : forall (t t':term) (a:gmargs), lcA a ->
+     ccRTT R t t' -> ccRTT R (app t a) (app t' a)
+ | cc_app2 : forall (t:term) (a a':gmargs), lcT t ->
+     ccRTA R a a' -> ccRTT R (app t a) (app t a')
+with ccRTA (R : term -> term -> Prop) : gmargs -> gmargs -> Prop :=    (* in gmargs *)
+ | cc_args1 : forall (u u':term) (l:alist) (c:cont), lcL l -> lcC c ->
+     ccRTT R u u' -> ccRTA R (args u l c) (args u' l c)
+ | cc_args2 : forall (u:term) (l l':alist) (c:cont), lcT u -> lcC c ->
+     ccRTL R l l' -> ccRTA R (args u l c) (args u l' c)
+ | cc_args3 : forall (u:term) (l:alist) (c c':cont), lcT u -> lcL l ->
+     ccRTC R c c' -> ccRTA R (args u l c) (args u l c')
+with ccRTL (R : term -> term -> Prop) : alist -> alist -> Prop :=     (* in alist *)
+ | cc_head : forall (u u':term) (l:alist) , lcL l ->
+     ccRTT R u u' -> ccRTL R (acons u l) (acons u' l)
+ | cc_tail : forall (u :term) (l l':alist) , lcT u ->
+     ccRTL R l l' -> ccRTL R (acons u l) (acons u l')
+with ccRTC (R : term -> term -> Prop) : cont -> cont -> Prop :=       (* in cont *)
+ | cc_cabs : forall (v v':term) (L:vars),
+     (forall (x:var), x `notin` L ->
+     ccRTT R (openT v (var_f x))  (openT v' (var_f x)))
+      -> ccRTC R (cabs v) (cabs v').
+
+
+Scheme ccRTT_ind_4 := Induction for ccRTT Sort Prop
+  with ccRTA_ind_4 := Induction for ccRTA Sort Prop
+  with ccRTL_ind_4 := Induction for ccRTL Sort Prop   
+  with ccRTC_ind_4 := Induction for ccRTC Sort Prop.
+
+
+Combined Scheme ccRT_mutind from
+         ccRTT_ind_4, ccRTA_ind_4, ccRTL_ind_4, ccRTC_ind_4.
+
+Definition ccBeta1T := ccRTT beta1T.
+
+
+(* Simulation of one step beta reduction ---with compatible closure --by one step beta1 of LJm *)
+
+
+Theorem sim_by_ccbeta_term : forall e1 e2,
+    ccBeta e1 e2 -> ccBeta1T  (exp_to_terms e1) (exp_to_terms e2).
 Proof.
-  intros e1 e2 H1 H2 H. induction H. inversion H1. subst.
-  unfold open_term_wrt_term in *. simpl in *. inversion H6.
-  rewrite (term_to_exp_commutes_open u t
-                                     (il_app_inv2 (abs t) u H1)
-                                     (il_abs_inv t (il_app_inv1 (abs t) u H1))).
-  apply beta_base.
-  - apply S.lc_abs. intro x.
-    change (S.lc_exp (open
-                        ((term_to_exp t) (il_abs_inv t (il_app_inv1 (abs t) u H1)))
-                        (term_to_exp (L.var_f x) (il_var_f x)))).
-    rewrite <- (term_to_exp_commutes_open _ _ _ _ (open_preserves_il (L.var_f x) 
-                                                                    t (il_var_f x) H5 0)).
-    apply term_to_exp_preserves_lc. inversion H. apply H9.
-  - apply term_to_exp_preserves_lc. apply H0.
+  intros. induction H.
+  - intros. constructor. apply sim_by_beta_term. assumption.
+  - simpl. apply cc_app1.
+    + constructor;eauto.
+      * eapply lcT_from_lc_exp. assumption.
+      * constructor. intro. cbn. auto.
+    + fold ccBeta1T. assumption.
+  - simpl. apply cc_app2.
+    + eapply lcT_from_lc_exp. assumption.
+    + constructor; eauto. constructor. intro. cbn. auto.
+  - simpl. apply cc_abs with (L:=L). intros.
+    change (ccRTT beta1T (openT (exp_to_terms e1) (exp_to_terms (S.var_f x)))
+                  (openT (exp_to_terms e2) (exp_to_terms (S.var_f x)))).
+    repeat (rewrite <- commut_opens).  fold ccBeta1T.  specialize (H0 x). auto. 
 Qed.
+
